James C - more high-level stuff

Jack/JackLanguage.thy
@@ -6,7 +6,7 @@ typedecl variable
 
 datatype type = 
   IntT | BoolT | CharT | UnitT 
-| ObjT variable "variable \<rightharpoonup> type" 
+| ObjT variable
 | ArrayT type 
 | ArrowT "type list" type
 
@@ -20,7 +20,8 @@ datatype expression =
 | BConst bool
 | CConst char
 | Var variable
-| This | Null
+| This 
+| Null
 | Index expression expression 
 | Field expression variable 
 | Call expression variable "expression list"
@@ -40,18 +41,34 @@ datatype statement =
 | Do expression variable "expression list"
 | Return expression
 
+record subroutine = 
+  outtype :: type
+  params :: "(variable \<times> type) list"
+  locals :: "(variable \<times> type) list"
+  body :: "statement list"
+
+record classdecl =
+  staticvars :: "(variable \<times> type) list" 
+  instancevars :: "(variable \<times> type) list"
+  staticfuncs :: "(variable \<times> subroutine) list"
+  instancefuncs :: "(variable \<times> subroutine) list"
+
+datatype program = Program "(variable \<times> classdecl) list" "statement list"
+
+(* typechecking *)
+
 inductive typecheck_binop :: "binop \<Rightarrow> type \<Rightarrow> type \<Rightarrow> bool" where
-  "typecheck_binop Plus IntT IntT"
-| "typecheck_binop Minus IntT IntT"
-| "typecheck_binop Times IntT IntT"
-| "typecheck_binop Div IntT IntT"
-| "typecheck_binop And BoolT BoolT"
-| "typecheck_binop Or BoolT BoolT"
-| "typecheck_binop Eq IntT BoolT"
-| "typecheck_binop Eq CharT BoolT"
-| "typecheck_binop Eq BoolT BoolT"
-| "typecheck_binop Gt IntT BoolT"
-| "typecheck_binop Lt IntT BoolT"
+  tc_plus [simp]: "typecheck_binop Plus IntT IntT"
+| tc_minus [simp]: "typecheck_binop Minus IntT IntT"
+| tc_times [simp]: "typecheck_binop Times IntT IntT"
+| tc_div [simp]: "typecheck_binop Div IntT IntT"
+| tc_and [simp]: "typecheck_binop And BoolT BoolT"
+| tc_or [simp]: "typecheck_binop Or BoolT BoolT"
+| tc_eqi [simp]: "typecheck_binop Eq IntT BoolT"
+| tc_eqc [simp]: "typecheck_binop Eq CharT BoolT"
+| tc_eqb [simp]: "typecheck_binop Eq BoolT BoolT"
+| tc_gt [simp]: "typecheck_binop Gt IntT BoolT"
+| tc_lt [simp]: "typecheck_binop Lt IntT BoolT"
 
 inductive typecheck_expr :: "(variable \<rightharpoonup> type) \<Rightarrow> type \<Rightarrow> expression \<Rightarrow> type \<Rightarrow> bool" where
   "typecheck_expr \<Gamma> this (IConst i) IntT"
@@ -59,11 +76,11 @@ inductive typecheck_expr :: "(variable \<rightharpoonup> type) \<Rightarrow> typ
 | "typecheck_expr \<Gamma> this (CConst b) CharT"
 | "\<Gamma> x = Some t \<Longrightarrow> typecheck_expr \<Gamma> this (Var x) t"
 | "typecheck_expr \<Gamma> this This this"
-| "typecheck_expr \<Gamma> this Null (ObjT that)"
+| "typecheck_expr \<Gamma> this Null (ObjT tx)"
 | "typecheck_expr \<Gamma> this e1 (ArrayT t) \<Longrightarrow> typecheck_expr \<Gamma> this e2 IntT \<Longrightarrow> 
     typecheck_expr \<Gamma> this (Index e1 e2) t"
-| "typecheck_expr \<Gamma> this e (ObjT that) \<Longrightarrow> that x = Some t \<Longrightarrow> typecheck_expr \<Gamma> this (Field e x) t"
-| "typecheck_expr \<Gamma> this e (ObjT that) \<Longrightarrow> that x = Some (ArrowT ts t) \<Longrightarrow> 
+| "typecheck_expr \<Gamma> this e (ObjT tx) \<Longrightarrow> badbadbad x = Some t \<Longrightarrow> typecheck_expr \<Gamma> this (Field e x) t"
+| "typecheck_expr \<Gamma> this e (ObjT tx) \<Longrightarrow> badbadbad x = Some (ArrowT ts t) \<Longrightarrow> 
     \<forall>(e', t') \<in> set (zip es ts). typecheck_expr \<Gamma> this e' t' \<Longrightarrow> 
       typecheck_expr \<Gamma> this (Call e x es) t"
 | "typecheck_expr \<Gamma> this e IntT \<Longrightarrow> typecheck_expr \<Gamma> this (Negate e) IntT"
@@ -75,7 +92,7 @@ inductive typecheck_lval :: "(variable \<rightharpoonup> type) \<Rightarrow> typ
   "\<Gamma> x = Some t \<Longrightarrow> typecheck_lval \<Gamma> this (LVar x) t"
 | "typecheck_lval \<Gamma> this l1 (ArrayT t) \<Longrightarrow> typecheck_expr \<Gamma> this e2 IntT \<Longrightarrow> 
     typecheck_lval \<Gamma> this (LIndex l1 e2) t"
-| "typecheck_lval \<Gamma> this e (ObjT that) \<Longrightarrow> that x = Some t \<Longrightarrow> typecheck_lval \<Gamma> this (LField e x) t"
+| "typecheck_lval \<Gamma> this e (ObjT tx) \<Longrightarrow> badbadbad x = Some t \<Longrightarrow> typecheck_lval \<Gamma> this (LField e x) t"
 
 inductive typecheck_stmt :: "(variable \<rightharpoonup> type) \<Rightarrow> type \<Rightarrow> type \<Rightarrow> statement \<Rightarrow> bool" where
   "typecheck_lval \<Gamma> this x t \<Longrightarrow> typecheck_expr \<Gamma> this e t \<Longrightarrow> typecheck_stmt \<Gamma> this out (Let x e)"
@@ -83,9 +100,20 @@ inductive typecheck_stmt :: "(variable \<rightharpoonup> type) \<Rightarrow> typ
     \<forall>s' \<in> set s2. typecheck_stmt \<Gamma> this out s' \<Longrightarrow> typecheck_stmt \<Gamma> this out (If e s1 s2)"
 | "typecheck_expr \<Gamma> this e BoolT \<Longrightarrow> \<forall>s' \<in> set s. typecheck_stmt \<Gamma> this out s' \<Longrightarrow> 
     typecheck_stmt \<Gamma> this out (While e s)"
-| "typecheck_expr \<Gamma> this e (ObjT that) \<Longrightarrow> that x = Some (ArrowT ts UnitT) \<Longrightarrow> 
+| "typecheck_expr \<Gamma> this e (ObjT tx) \<Longrightarrow> badbadbad x = Some (ArrowT ts UnitT) \<Longrightarrow> 
     \<forall>(e', t') \<in> set (zip es ts). typecheck_expr \<Gamma> this e' t' \<Longrightarrow> 
       typecheck_stmt \<Gamma> this out (Do e x es)"
 | "typecheck_expr \<Gamma> this e out \<Longrightarrow> typecheck_stmt \<Gamma> this out (Return e)"
+
+inductive typecheck_subr :: "(variable \<rightharpoonup> type) \<Rightarrow> type \<Rightarrow> subroutine \<Rightarrow> bool" where
+  "\<forall>s \<in> set sts. typecheck_stmt (\<Gamma> ++ map_of ps ++ map_of ls) this t s \<Longrightarrow> 
+    typecheck_subr \<Gamma> this \<lparr> outtype = t, params = ps, locals = ls, body = sts \<rparr>"
+
+inductive typecheck_class :: "classdecl \<Rightarrow> bool" where
+  "typecheck_class \<lparr> staticvars = svs, instancevars = ivs, staticfuncs = sfs, instancefuncs = ifs \<rparr>"
+
+inductive typecheck_program :: "program \<Rightarrow> bool" where
+  "\<forall>(n, cl) \<in> set classes. typecheck_class cl \<Longrightarrow> \<forall>s \<in> set main. typecheck_stmt \<Gamma> this t s \<Longrightarrow> 
+    typecheck_program (Program classes main)"
 
 end
